wip: proving termination of ext traces

fairness/examples/comp/comp_adequacy.v
@@ -1,23 +1,24 @@
 From iris.proofmode Require Import tactics.
-From trillium.program_logic Require Export weakestpre.
-From trillium.prelude Require Export finitary quantifiers sigma classical_instances.
+From trillium.program_logic Require Import weakestpre.
+From trillium.prelude Require Import finitary quantifiers sigma classical_instances.
 Require Import stdpp.decidable.
-From trillium.fairness.heap_lang Require Export lang lifting tactics proofmode.
+From trillium.fairness.heap_lang Require Import lang lifting tactics proofmode.
 From trillium.fairness.heap_lang Require Import notation.
-From trillium.fairness.heap_lang Require Import simulation_adequacy_lm.
+From trillium.fairness.heap_lang Require Import simulation_adequacy_lm simulation_adequacy_lm_ext.
 From iris.base_logic.lib Require Import invariants.
 From iris.prelude Require Import options.
 From iris.algebra Require Import excl_auth.
 From iris.bi Require Import bi.
 From stdpp Require Import finite.
-From trillium.fairness Require Import fairness_finiteness lm_lsi_top. 
+From trillium.fairness Require Import fairness_finiteness lm_lsi_top resources. 
 
 Import derived_laws_later.bi.
 
-From trillium.fairness Require Import lm_fairness_preservation fuel_ext lm_fair.
-From trillium.fairness.examples.comp Require Import comp lib.
+From trillium.fairness Require Import lm_fairness_preservation fuel_ext lm_fair lm_fair_traces fair_termination.
+From trillium.fairness.ext_models Require Import destutter_ext ext_models.
+From trillium.fairness.examples.comp Require Import comp lib lib_ext. 
 From trillium.fairness Require Import fair_termination_natural.
-From trillium.fairness.examples.comp Require Import my_omega lemmas trace_len trace_helpers subtrace trace_lookup.
+From trillium.fairness Require Import my_omega lemmas trace_len trace_helpers subtrace trace_lookup.
 
 From trillium.fairness Require Import lm_fairness_preservation_wip.
 
@@ -158,7 +159,7 @@ Proof.
   pose proof STEP0 as (atr & AFTER & HEAD)%trace_lookup_after_strong.
   apply after_S_tr_cons in AFTER. 
   specialize (IHc0 δ1 atr). specialize_full IHc0; eauto. 
-  { eapply mtrace_valid_after; eauto. }
+  { eapply trace_valid_after; eauto. }
   { intros. apply (CL (S i)). rewrite -H.
     symmetry. rewrite -Nat.add_1_r Nat.add_comm.
     eapply trace_lookup_after; eauto. }
@@ -273,24 +274,30 @@ Proof. Admitted.
   
 
 
-CoFixpoint project_lib_trace (tr: mtrace client_model_impl):
-  auxtrace (LM := lib_model). 
-destruct tr.
-{ exact ⟨ fst s ⟩. }
-(* cases not corresponding to library role
-   should be ruled out during actual construction *)
-destruct ℓ.
-2: { exact ⟨ fst s ⟩. }
-destruct f.
-2: { exact ⟨ fst s ⟩. }
-set (fls := allowed_step_FLs (fst s) f (fst $ trfirst tr) (LM := lib_model)).
-destruct (decide (fls = ∅)).
-{ exact ⟨ fst s ⟩. }
-assert (elements fls ≠ []).
-{ intros ?%elements_empty_inv. set_solver. }
-destruct (elements fls) eqn:ELS; [done| ]. 
-exact ((fst s) -[f0]-> (project_lib_trace tr)).
-Defined. 
+CoFixpoint project_lib_trace (tr: mtrace client_model_impl): 
+  elmftrace (ELM := ExtLibLM)
+  (* @atrace _ _ _ lib_model (option $ ext_role (EM := ExtLibLM)) *)
+  :=
+  match tr with 
+  | ⟨ s ⟩ => ⟨ fst s ⟩
+  | s -[Some (inl l)]-> tr' => (fst s) -[ Some l ]-> (project_lib_trace tr')
+  | s -[ _ ]-> tr' => ⟨fst s ⟩
+  end. 
+
+Lemma project_lib_trfirst (tr: mtrace client_model_impl):
+    trfirst (project_lib_trace tr) = fst (trfirst tr).
+Proof. 
+  destruct tr; eauto.
+  destruct ℓ; [destruct f|]; eauto. 
+Qed. 
+
+(* CoFixpoint project_lib_trace (tr: mtrace client_model_impl): elmftrace (ELM := ExtLibLM) := *)
+(*   match tr with  *)
+(*   | ⟨ s ⟩ => ⟨ fst s ⟩ *)
+(*   | s -[Some (inl ρlg)]-> tr' => (fst s) -[ Some $ inl ρlg ]-> (project_lib_trace tr') *)
+(*   | s -[ _ ]-> tr' => ⟨fst s ⟩ *)
+(*   end.  *)
+
 
 Definition is_end_state (step: client_state * option (option client_role * client_state)) :=
   exists st, step = (st, None). 
@@ -299,7 +306,8 @@ Lemma lib_trace_construction (tr: mtrace client_model_impl)
   (VALID: mtrace_valid tr)
   (LIB_STEPS: ∀ i res, tr !! i = Some res → is_lib_step res \/ is_end_state res):
     lm_model_traces_match
-      (inl: lib_grole -> fmrole client_model_impl)
+      (transA := @ext_trans _ ExtLibLM)
+      ((option_fmap _ _ inl): option (@ext_role _ ExtLibLM) -> option $ fmrole client_model_impl)
       (fun c δ_lib => fst c = δ_lib)
       tr
       (project_lib_trace tr).
@@ -307,28 +315,58 @@ Proof.
   gd tr. cofix IH.
   intros. 
   rewrite (trace_unfold_fold (project_lib_trace tr)).
-  rewrite /project_lib_trace.
   destruct tr.
   { econstructor. done. }
   do 2 red.
   pose proof (LIB_STEPS 0 (s, Some (ℓ, (trfirst tr))) eq_refl) as STEP0.
   destruct STEP0 as [STEP0 | STEP0].
   2: { destruct STEP0. done. }
-  destruct STEP0 as (?&?&?&[=]&[ρlg <-]). subst. simpl in *. 
-  destruct decide.
-  { forward eapply (mtrace_valid_steps' VALID 0) as TRANS0; [eauto| ]. 
-    inversion TRANS0; subst. 
-    eapply locale_trans_alt in LIB_STEP.
-    by rewrite -H2 in e. }
-Admitted. 
+  (* pose proof (trace_valid_cons_inv _ _ _ _ VALID) as [VALID' STEP].   *)
+  destruct STEP0 as (?&?&?&[=]&[ρlg <-]). subst. simpl in *.
+  econstructor.
+  1-3: done.
+  { rewrite project_lib_trfirst. inversion STEP; subst; simpl in *.
+    all: rewrite -H2; econstructor; eauto. }
+  eapply IH; eauto. intros. 
+  apply (LIB_STEPS (S i)); eauto. 
+Qed.
 
+Local Lemma client_lr_0_tmp δ:
+  client_lr (δ, 0) = ∅.
+Proof. Admitted. 
+
+(* TODO: abstract the nested LM state *)
+Local Instance inh_client: Inhabited (lm_ls client_model).
+Proof.
+  assert (Inhabited (lm_ls lib_model)) as [δ] by apply _.
+  assert (Inhabited (locale heap_lang)) as [τ] by apply _.
+  apply populate.
+  refine {| ls_under := (δ, 0): fmstate client_model_impl;
+       ls_fuel := kmap (inl ∘ inl) (gset_to_gmap 0 (dom (ls_tmap δ)));
+       ls_mapping := kmap (inl ∘ inl) (gset_to_gmap τ (dom (ls_tmap δ)));
+    |}.
+  Unshelve.
+  - simpl. rewrite client_lr_0_tmp. set_solver. 
+  - apply leibniz_equiv. rewrite !dom_kmap.
+    f_equiv. by rewrite !dom_gset_to_gmap. 
+  - red. intros gi IN.
+    rewrite dom_kmap. apply elem_of_map. eexists. split; eauto.
+    rewrite dom_gset_to_gmap.
+    destruct IN as [? IN]. apply (ls_mapping_tmap_corr (LM := lib_model)) in IN.
+    destruct IN as (?&?&?). simpl in *.
+    eapply elem_of_dom; eauto. 
+Qed. 
+
+Local Instance client_LF: LMFairPre client_model.
+  esplit; apply _.
+Qed. 
 
 Definition outer_LM_trace_exposing
-  (lmtr: auxtrace (LM := client_model)) (mtr: mtrace client_model_impl) :=
+  (lmtr: lmftrace (LM := client_model)) (mtr: mtrace client_model_impl) :=
   upto_stutter_auxtr lmtr mtr /\
-  (∀ n gi, fair_aux_SoU lmtr (inl gi) n) /\
+  (∀ gi, fair_aux_SoU _ ((inl $ inl gi): fmrole client_model_impl) lmtr) /\
   (* TODO: remove LMo parameter from inner_obls_exposed *)
-  inner_obls_exposed inl (λ c δ_lib, c.1 = δ_lib) lmtr (LMo := client_model).
+  inner_obls_exposed (inl ∘ inl) (λ c δ_lib, c.1 = δ_lib) lmtr (LMo := client_model).
 
 Definition traces_equiv {St L: Type} :=
   @traces_match L L St St eq eq (fun _ _ _ => True) (fun _ _ _ => True).
@@ -411,9 +449,9 @@ Qed.
 
 
 From Paco Require Import paco1 paco2 pacotac.
-Lemma upto_stutter_Proper_impl {St S' L L': Type} {Us: St -> S'} {Ul: L -> option L'}:
+Lemma upto_stutter_Proper_impl {St S' L L': Type} {Us: St -> S'} {Usls: St -> L -> St -> option L'}:
   Proper (@traces_equiv St L ==> @traces_equiv S' L' ==> impl)
-    (upto_stutter Us Ul).
+    (upto_stutter Us Usls).
 Proof. 
   red. intros t1 t1' EQ1 t2 t2' EQ2 UPTO.
   gd t1. gd t2. gd t1'. gd t2'.
@@ -449,16 +487,16 @@ Proof.
            (* all: admit. } *)
 Admitted. 
 
-Instance upto_stutter_Proper {St S' L L': Type} {Us: St -> S'} {Ul: L -> option L'}:
+Instance upto_stutter_Proper {St S' L L': Type} {Us: St -> S'} {Usls: St -> L -> St -> option L'}:
   Proper (@traces_equiv St L ==> @traces_equiv S' L' ==> iff)
-    (upto_stutter Us Ul).
+    (upto_stutter Us Usls).
 Proof. 
   red. intros ??????. split.
   - intros. eapply upto_stutter_Proper_impl; eauto.
   - intros. apply traces_equiv_symm in H, H0. 
     eapply upto_stutter_Proper_impl; eauto.
-Qed. 
-                                   
+Qed.
+
 
 Lemma outer_exposing_subtrace ltr tr i str 
   (OUTER_CORR: outer_LM_trace_exposing ltr tr)
@@ -476,7 +514,7 @@ Proof.
     + reflexivity. 
     + by symmetry.
   - intros.
-    forward eapply fair_aux_SoU_after; [| apply AFTER' |]; eauto.
+    forward eapply fair_by_gen_after; [apply AFTER' |..]; eauto.
     intros. apply FAIR_AUX.
   - eapply inner_obls_exposed_after; eauto.
 Qed.   
@@ -509,7 +547,7 @@ Lemma client_trace_lookup (tr: mtrace client_model_impl) i
   terminating_trace tr \/
   exists step, tr !! i = Some step /\
             (is_client_step step \/
-             is_lib_step step /\ snd $ fst step = 1).
+             is_lib_step step /\ (snd $ fst step = 2 \/ snd $ fst step = 1)).
 Proof.
   pose proof (trace_has_len tr) as [len LEN].
   destruct (tr !! i) as [[st step]|] eqn:ST.
@@ -522,10 +560,9 @@ Proof.
   right. eexists. split; eauto. simpl.
   forward eapply (mtrace_valid_steps' VALID i) as TRANS; [eauto| ].
   simpl in TRANS.
-  inversion TRANS; subst.
-  1, 3: left; do 2 red; eauto.
-  right. split; eauto. do 2 red.
-  do 3 eexists. eauto.
+  inversion TRANS; subst; simpl.
+  1, 4: by (left; do 2 red; eauto). 
+  all: right; split; eauto; do 2 red; do 3 eexists; eauto. 
 Qed. 
 
 (* TODO: try to unify with 'kept_*' lemmas
@@ -578,7 +615,9 @@ Proof.
   eapply preserved_prop_kept; eauto.
   intros ??? LIB STEP EQ1.
   do 2 red in LIB. destruct LIB as (?&?&?&[=]&[? <-]). subst.
-  simpl in STEP. inversion STEP. by subst.
+  simpl in STEP. inversion STEP.
+  - by subst.
+  - by simpl in *.
 Qed.
 
 (* TODO: inline? *)  
@@ -605,7 +644,7 @@ Proof.
   (* destruct (infinite_or_finite tr) as [INF|]; [| done]. *)
   pose proof (trace_has_len tr) as [len LEN]. 
 
-  assert (len = NOnum 1 \/ NOmega.lt_nat_l 1 len /\ snd (trfirst tr) <= 2) as [-> | [LENnz BOUNDc]].
+  assert (len = NOnum 1 \/ NOmega.lt_nat_l 1 len /\ snd (trfirst tr) <= 3) as [-> | [LENnz BOUNDc]].
   { pose proof (trace_lookup_0_Some tr) as [[δ0 step0] STEP0].
     destruct step0.
     2: { left. rewrite -(plus_O_n 1).
@@ -622,9 +661,7 @@ Proof.
   forward eapply (trace_prop_split tr is_client_step) as [l1 (L1 & NL1 & DOM1)]; eauto.
   { eapply slm_dec. intros.
     (* TODO: why it's not inferred automatically? *)
-    assert (EqDecision client_role).    
-    { apply (@sum_eq_dec (fmrole lib_fair) lib_role_EqDec y_role y_EqDec). } 
-    solve_decision. }
+    unshelve eapply sum_eq_dec. solve_decision. }
 
   (* assert (exists n1, l1 = NOnum n1 /\ (forall s, tr S!! (n1 - 1) = Some s -> snd s < 2)) as (m1 & LEN1 & BOUNDc').  *)
   assert (exists n1, l1 = NOnum n1) as (m1 & LEN1).
@@ -648,10 +685,7 @@ Proof.
   forward eapply (trace_prop_split' tr is_lib_step _ m1)
     as (l2 & L2 & NL2 & LE2 & LE2'); eauto.
   { eapply slm_dec. intros.
-    (* TODO: why it's not inferred automatically? *)
-    assert (EqDecision client_role).    
-    { apply (@sum_eq_dec (fmrole lib_fair) lib_role_EqDec y_role y_EqDec). } 
-    solve_decision. }
+    destruct ρ; [left | right]; eauto. by intros [??]. }
 
   assert (exists m2, l2 = NOnum m2) as [m2 ->].
   { destruct l2 eqn:L2_EQ; [| by eauto].
@@ -674,8 +708,12 @@ Proof.
     (* 3: { Unshelve. *)
     (*   apply MATCH.  *)
 
-    eapply simulation_adequacy_terminate_general' in MATCH; eauto; cycle 1. 
-    { apply lib_fair_term. }
+    (* forward eapply (simulation_adequacy_terminate_general'_ext str (project_lib_trace str)). *)
+    (* 4: { apply MATCH.  *)
+    eapply @simulation_adequacy_terminate_general'_ext in MATCH; eauto; cycle 1. 
+    (* eapply simulation_adequacy_terminate_general'_ext in MATCH; eauto; cycle 1.  *)
+    { exact (lib_lm_projEI: @EI _ ExtLibLM -> @EI _ ExtLib). }  
+    {  apply lib_fair_term. }
     {       
       subst. simpl in *.
       forward eapply outer_exposing_subtrace; eauto.
