fairness/ext_models/ext_models.v
@@ -1,6 +1,6 @@
 From trillium.fairness Require Import fairness fair_termination.
 From trillium.fairness.examples.ticketlock Require Import set_map_properties. 
-From trillium.fairness Require Import trace_helpers lm_fairness_preservation lm_fair fuel.
+From trillium.fairness Require Import trace_helpers lm_fairness_preservation lm_fair fuel trace_len.
 
 Class ExtModel (innerM: FairModel) := {  
   EI: Type; (* indexes over external transitions *)
@@ -76,6 +76,148 @@ Section ExtModelFair.
   Definition emtrace_valid := trace_valid ext_trans. 
 
 End ExtModelFair. 
+
+
+Definition trans_bounded {St L: Type} (tr: trace St L) (P: L -> Prop) :=
+  exists n, forall i ℓ, n <= i -> tr L!! i = Some ℓ -> ¬ P ℓ.
+
+Lemma fin_trans_bounded {St L: Type} (tr: trace St L) (P: L -> Prop)
+  (FIN: terminating_trace tr):
+  trans_bounded tr P.
+Proof.
+  pose proof (trace_has_len tr) as [? LEN].
+  eapply terminating_trace_equiv in FIN as [n ?]; eauto. subst. 
+  red. exists n. intros.
+  eapply mk_is_Some, label_lookup_dom in H0; eauto.
+  simpl in *. lia.
+Qed. 
+
+Section TraceProjection.
+  Context {St L St' L': Type}.
+  Context (proj_st: St -> St'). 
+  Context (proj_lbl: L -> option L'). 
+
+  CoFixpoint project_trace_until (tr: trace St L): trace St' L'
+  (* @atrace _ _ _ lib_model (option $ ext_role (EM := ExtLibLM)) *)
+  :=
+  match tr with 
+  | ⟨ s ⟩ => ⟨ proj_st s ⟩
+  | s -[ℓ]-> tr' => match (proj_lbl ℓ) with
+                  | Some l => (proj_st s) -[ l ]-> (project_trace_until tr')
+                  | None => ⟨ proj_st s ⟩
+                  end
+  end. 
+
+  Lemma project_until_trfirst (tr: trace St L):
+    trfirst (project_trace_until tr) = proj_st (trfirst tr).
+  Proof. 
+    destruct tr; eauto. simpl. 
+    destruct (proj_lbl ℓ); eauto. 
+  Qed. 
+
+  Lemma project_until_match (tr: trace St L)
+    (trans: St -> L -> St -> Prop) (trans': St' -> L' -> St' -> Prop)
+    (VALID: trace_valid trans tr)
+    (STEP_KEPT: forall s1 ℓ s2 l, trans s1 ℓ s2 -> proj_lbl ℓ = Some l -> trans' (proj_st s1) l (proj_st s2))
+    (PROJ: forall i ℓ, tr L!! i = Some ℓ -> exists l, proj_lbl ℓ = Some l):
+    traces_match
+      (fun ℓ l => proj_lbl ℓ = Some l) (fun s s' => proj_st s = s')
+      trans trans'
+      tr (project_trace_until tr).
+  Proof.
+    generalize dependent tr. cofix IH.
+    intros. 
+    rewrite (trace_unfold_fold (project_trace_until tr)).
+    destruct tr.
+    { econstructor. done. }
+    apply trace_valid_cons_inv in VALID as [VALID' STEP]. 
+    pose proof (PROJ 0 ℓ ltac:(done)) as [l LBL].
+    simpl. rewrite LBL. 
+    econstructor; try done.
+    { rewrite project_until_trfirst. eapply STEP_KEPT; eauto. }
+    eapply IH; eauto.
+    intros. by apply (PROJ (S i)).
+  Qed. 
+
+End TraceProjection.
+
+Section ExtTerm.
+  Context `{EM: ExtModel M}. 
+
+  (* TODO: move *)
+  Lemma terminating_trace_after {St L: Type} (tr atr: trace St L) i
+    (AFTER: after i tr = Some atr)
+    (FIN_ATR: terminating_trace atr):
+    terminating_trace tr.
+  Proof.
+    destruct FIN_ATR as [n FIN].
+    exists (i + n). by rewrite after_sum' AFTER.
+  Qed. 
+
+  Definition ext_trans_bounded (emtr: emtrace) :=
+    trans_bounded emtr (fun oℓ => exists ι, oℓ = Some (inr ι)). 
+ 
+  Lemma fin_ext_fair_termination (emtr : emtrace)
+    (VALID: emtrace_valid emtr)
+    (EXT_BOUND: ext_trans_bounded emtr)
+    (FAIR: inner_fair_ext_model_trace emtr)
+    (FAIR_TERM_INNER: forall mtr, @mtrace_fairly_terminating M mtr):
+    terminating_trace emtr.
+  Proof.
+    do 2 red in EXT_BOUND. destruct EXT_BOUND as [n BOUND].
+    destruct (after n emtr) as [atr| ] eqn:AFTER.
+    2: { by exists n. }
+    eapply terminating_trace_after; eauto.
+    eapply trace_valid_after in VALID; eauto.
+    (* set (proj_ext := fun oℓ =>  *)
+    unshelve eapply project_until_match in VALID.
+    5: exact (fmtrans M). 
+    { exact (fun oer => match oer with | Some (inl g) => Some $ Some g | _ => None end). }
+    { exact id. }
+    2: { simpl. intros. destruct ℓ; simpl in *; try done.
+         destruct e; try done. 
+         inversion H0. subst. inversion H. congruence. }
+    2: { intros. erewrite label_lookup_after in H; eauto.
+         apply BOUND in H; [| lia].
+         assert (ℓ ≠ None).
+         { (* exploit emtr validity.
+              Generalize trace_helpers.mtrace_valid_steps'' for that
+            *)
+           admit. }
+         destruct ℓ; [| congruence].
+         destruct e; eauto.
+         edestruct H; eauto. }
+    remember (project_trace_until _ _ _) as mtr. clear Heqmtr. 
+    eapply traces_match_preserves_termination; eauto.
+    apply FAIR_TERM_INNER.
+    { eapply traces_match_valid2; eauto. }
+    intros. do 2 red. intros k ENk. 
+    specialize (FAIR (inl ρ)). simpl in FAIR. specialize (FAIR ltac:(eauto)).
+    do 2 red in FAIR. specialize (FAIR (n + k)). destruct FAIR.
+    { apply pred_at_trace_lookup. apply pred_at_trace_lookup in ENk as (?&KTH&?).
+      eexists. split.
+      { eapply traces_match_state_lookup_2 in KTH as (?&?&?); [| by eauto].
+        simpl in *. subst. 
+        erewrite <- state_lookup_after; eauto. }
+      red. simpl. rewrite /ext_live_roles. set_solver. }
+    exists x. apply pred_at_trace_lookup. apply pred_at_trace_lookup in H as (?&NEXT&STEP).
+    eexists. split.
+    { rewrite -Nat.add_assoc in NEXT. 
+      erewrite <- state_lookup_after in NEXT; eauto. 
+      eapply traces_match_state_lookup_1 in NEXT as (?&?&?); [| by eauto].
+      simpl in *. subst. by rewrite H. }
+    red in STEP. destruct STEP as [DIS | STEP].
+    { left. intros ?. apply DIS.
+      red. simpl. rewrite /ext_live_roles. set_solver. }
+    right.
+    foobar. 
+    
+    
+    
+         
+    
+
+End ExtTerm.
 
 (* TODO: move? *)
 Section ELM_ALM.
